Rename [cif] to [Fml]

src/Iris/Nola/Embedding.lean
@@ -5,7 +5,7 @@ import Iris.Nola.Inv
 
 inductive AProp.{u} FF : Bool -> Type _ where
 | IProp (P : Iris.IProp FF) : AProp FF true
-| FProp (fP : cif.{u} FF) : AProp FF false
+| FProp (fP : Fml.{u} FF) : AProp FF false
 
 namespace AProp
 
@@ -14,18 +14,18 @@ def to_IProp : AProp FF b -> Iris.IProp FF
 | FProp P => ⟦ P ⟧
 
 def guard : AProp FF b -> AProp FF false
-| IProp P => FProp cif(▷ P)
+| IProp P => FProp fml(▷ P)
 | FProp P => FProp P
 
 def unguard : AProp FF b -> AProp FF true
 | IProp P => IProp P
 | FProp P => IProp ⟦ P ⟧
 
-def to_Formula : AProp FF b -> cif FF := fun P =>
+def to_Formula : AProp FF b -> Fml FF := fun P =>
 match P.guard with
 | FProp fP => fP
 
-def of_Formula (F : cif.{u} FF) : AProp.{u} FF false :=
+def of_Formula (F : Fml.{u} FF) : AProp.{u} FF false :=
   FProp F
 
 /- Binary connectives -/
@@ -35,35 +35,35 @@ match P, Q with
 | IProp P, IProp Q => IProp iprop(P ∧ Q)
 | IProp P, FProp Q => IProp iprop(P ∧ ⟦Q⟧)
 | FProp P , IProp Q => IProp iprop(⟦P⟧ ∧ Q)
-| FProp P, FProp Q => FProp cif(P ∧ Q)
+| FProp P, FProp Q => FProp fml(P ∧ Q)
 
 def or {b₁ b₂} (P : AProp FF b₁) (Q : AProp FF b₂) : AProp FF (b₁ || b₂) :=
 match P, Q with
 | IProp P, IProp Q => IProp iprop(P ∨ Q)
 | IProp P, FProp Q => IProp iprop(P ∨ ⟦Q⟧)
 | FProp P, IProp Q => IProp iprop(⟦P⟧ ∨ Q)
-| FProp P, FProp Q => FProp cif(P ∨ Q)
+| FProp P, FProp Q => FProp fml(P ∨ Q)
 
 def imp {b₁ b₂} (P : AProp FF b₁) (Q : AProp FF b₂) : AProp FF (b₁ || b₂) :=
 match P, Q with
 | IProp P, IProp Q => IProp iprop(P -> Q)
 | IProp P, FProp Q => IProp iprop(P -> ⟦Q⟧)
 | FProp P, IProp Q => IProp iprop(⟦P⟧ -> Q)
-| FProp P, FProp Q => FProp cif(P -> Q)
+| FProp P, FProp Q => FProp fml(P -> Q)
 
 def sep {b₁ b₂} (P : AProp FF b₁) (Q : AProp FF b₂) : AProp FF (b₁ || b₂) :=
 match P, Q with
 | IProp P, IProp Q => IProp iprop(P ∗ Q)
 | IProp P, FProp Q => IProp iprop(P ∗ ⟦Q⟧)
 | FProp P, IProp Q => IProp iprop(⟦P⟧ ∗ Q)
-| FProp P, FProp Q => FProp cif(P ∗ Q)
+| FProp P, FProp Q => FProp fml(P ∗ Q)
 
 def wand {b₁ b₂} (P : AProp FF b₁) (Q : AProp FF b₂) : AProp FF (b₁ || b₂) :=
 match P, Q with
 | IProp P, IProp Q => IProp iprop(P -∗ Q)
 | IProp P, FProp Q => IProp iprop(P -∗ ⟦Q⟧)
 | FProp P, IProp Q => IProp iprop(⟦P⟧ -∗ Q)
-| FProp P, FProp Q => FProp cif(P -∗ Q)
+| FProp P, FProp Q => FProp fml(P -∗ Q)
 
 theorem wandIff_all (A : Type) (P Q : A -> Iris.IProp FF) :
   (∀ (a : A), ⊢ iprop(P a ∗-∗ Q a)) ->
@@ -90,62 +90,45 @@ theorem wandIff_ex (A : Type) (P Q : A -> Iris.IProp FF) :
 
 def persistently {b} : AProp FF b -> AProp FF b
 | IProp P => IProp iprop(<pers> P)
-| FProp P => FProp cif(<pers> P)
+| FProp P => FProp fml(<pers> P)
 
 def plainly {b} : AProp FF b -> AProp FF b
 | IProp P => IProp iprop(■ P)
-| FProp P => FProp cif(■ P)
+| FProp P => FProp fml(■ P)
 
 def later {b} : AProp FF b -> AProp FF false
-| IProp P => FProp cif(▷ P)
-| FProp P => FProp cif(▷ ⟦P⟧)
+| IProp P => FProp fml(▷ P)
+| FProp P => FProp fml(▷ ⟦P⟧)
 
 def bupd {b} : AProp FF b -> AProp FF b
 | IProp P => IProp iprop(|==> P)
-| FProp P => FProp cif(|==> P)
+| FProp P => FProp fml(|==> P)
 
 def pure (P : Prop) : AProp FF false :=
-  FProp cif(⌜P⌝)
+  FProp fml(⌜P⌝)
 
 /- Quantifiers -/
 
-def all {A : Type} {b} (Φ : A -> AProp FF b) : AProp FF b :=
+set_option pp.universes true
+
+def all.{u} {A : Type u} {b} (Φ : A -> AProp.{u} FF b) : AProp.{u} FF b :=
 match b with
 | true => IProp iprop(∀ a, (Φ a).to_IProp)
-| false => FProp cif(∀ a, (Φ a).to_Formula)
+| false => FProp fml(∀ (a : A), (Φ a).to_Formula)
+
+def impred_all.{u, v} {A : Type u} (Φ : A -> AProp.{u} FF b) : AProp.{v} FF true :=
+  IProp iprop(∀ a, (Φ a).to_IProp)
 
 def all_pred {A : Type} (Φ : A -> (∀ b, AProp FF b)) : AProp FF true :=
   IProp iprop(∀ a, (Φ a true).to_IProp)
 
-noncomputable def cif.sForall.{u} (Φ : cif.{u} FF → Prop) : cif.{u} FF :=
-  cif(∀ (p : ULift (Iris.IProp FF)),
-      let fp : cif.{u} FF := Classical.epsilon (fun fp => (⊢ iprop(⟦ (fp) ⟧ ∗-∗ p.down)) ∧ Φ fp)
-      cif(⌜(⊢ ⟦ fp ⟧ ∗-∗ p.down) ∧ Φ fp⌝ -> fp))
-      -- cif.imp (cif.pure ((⊢ iprop(⟦ (fp) ⟧ ∗-∗ p.down)) ∧ Φ fp)) fp)
-
-  -- )
-  -- @cif.all.{u} FF (ULift (Iris.IProp FF)) (
-  --   fun (p : ULift (Iris.IProp FF)) =>
-  --   let fp : cif.{u} FF := Classical.epsilon (fun fp => ⊢ iprop(⟦ (fp) ⟧ ∗-∗ p.down))
-  --   cif.imp (cif.pure ((⊢ iprop(⟦ (fp) ⟧ ∗-∗ p.down)) ∧ Φ fp)) fp)
+noncomputable def Fml.sForall.{u} (Φ : Fml.{u} FF → Prop) : Fml.{u} FF :=
+  fml(∀ (p : ULift (Iris.IProp FF)),
+      let fp : Fml.{u} FF := Classical.epsilon (fun fp => (⊢ iprop(⟦ (fp) ⟧ ∗-∗ p.down)) ∧ Φ fp)
+      fml(⌜(⊢ ⟦ fp ⟧ ∗-∗ p.down) ∧ Φ fp⌝ -> fp))
 
 noncomputable def sForall (Ψ : AProp FF false -> Prop) : AProp FF false :=
-  FProp (AProp.cif.sForall (fun (p : cif FF) => Ψ (AProp.of_Formula p)))
-
--- def sForall (Ψ : AProp.{u + 1} FF false -> Prop) : AProp.{u+1} FF false :=
---   FProp
---     iprop(∀ (p : cif.{u} FF), ⌜Ψ (AProp.of_Formula (liftCif.{u,u+1} p))⌝ → ⟦ p ⟧)
---     cif(∀ (p : cif.{u} FF), ⌜Ψ (AProp.of_Formula (liftCif.{u,u+1} p))⌝ -> (liftCif.{u,u+1} p))
---     (by
---       simp [cif.sem, cif.sForall, cif.imp]
---       apply Iris.BI.equiv_wandIff
---       constructor <;> iintro H P HΨ
---       · ispecialize H P HΨ
---         istop; apply Iris.BI.entails_trans.trans Iris.BI.emp_sep.1
---         apply (cif.sem_lift _ _).1
---       · ispecialize H P HΨ
---         istop; apply Iris.BI.entails_trans.trans Iris.BI.emp_sep.1
---         apply (cif.sem_lift _ _).2)
+  FProp (AProp.Fml.sForall (fun (p : Fml FF) => Ψ (AProp.of_Formula p)))
 
 def sForall' {FF} (Ψ : AProp.{u+1} FF true -> Prop) : AProp.{u+1} FF true :=
   IProp (UPred.sForall (fun P => Ψ (IProp P)))
@@ -155,18 +138,18 @@ def sForall'' {FF} (Ψ : ∀ b, AProp FF b -> Prop) : AProp FF true :=
 
 def sExists (Ψ : AProp.{u+1} FF false -> Prop) : AProp.{u+1} FF false :=
   FProp
-    (cif.sExists.{u} (fun (p : cif.{u} FF) => Ψ (AProp.of_Formula (liftCif.{u,u+1} p))))
+    (Fml.sExists.{u} (fun (p : Fml.{u} FF) => Ψ (AProp.of_Formula (liftFml.{u,u+1} p))))
 
 def ex {A : Type} {b} (Φ : A -> AProp FF b) : AProp FF b :=
 match b with
 | true => IProp iprop(∃ a, (Φ a).to_IProp)
-| false => FProp cif(∃ (a : A), (Φ a).to_Formula)
+| false => FProp fml(∃ (a : A), (Φ a).to_Formula)
 
 def ex_pred {A : Type} (Φ : A -> (∀ b, AProp FF b)) : AProp FF true :=
   IProp iprop(∃ a, (Φ a true).to_IProp)
 
 def ainv_tok {b} (N : Namespace) (P : AProp FF b) : AProp FF false :=
-  FProp (cif.inv N P.to_Formula)
+  FProp (Fml.inv N P.to_Formula)
 -- theorem ainv_tok_alloc N (P : AProp FF b) :
 --   ⊢ iprop(P.to_IProp -∗ bupdw (inv_wsat) (ainv_tok N P))
 
