src/Iris/Nola/Inv.lean
@@ -12,23 +12,23 @@ import Iris.Nola.Syntax
 
 section sinv
 
-axiom sinv_tok (i : Pos) (F : cif FF) : Iris.IProp FF
+axiom sinv_tok (i : Pos) (F : Fml FF) : Iris.IProp FF
 
-axiom sinv_tok_lift (i : Pos) (F : cif FF) :
-  sinv_tok i (liftCif F) ⊣⊢ sinv_tok i F
+axiom sinv_tok_lift (i : Pos) (F : Fml FF) :
+  sinv_tok i (liftFml F) ⊣⊢ sinv_tok i F
 
-axiom sinv_auth_tok (M : List (cif FF)) : Iris.IProp FF
+axiom sinv_auth_tok (M : List (Fml FF)) : Iris.IProp FF
 
-def sinv_wsat (sm : cif FF -> Iris.IProp FF) : Iris.IProp FF :=
+def sinv_wsat (sm : Fml FF -> Iris.IProp FF) : Iris.IProp FF :=
   iprop(∃ M, sinv_auth_tok M ∗ [∗] (List.map (fun F => (sm F)) M))
 
-axiom sinv_wsat_timeless (sm : cif FF -> Iris.IProp FF) :
+axiom sinv_wsat_timeless (sm : Fml FF -> Iris.IProp FF) :
   Iris.BI.Timeless (sinv_wsat sm)
 
-axiom sinv_auth_tok_alloc (M : List (cif FF)) F :
+axiom sinv_auth_tok_alloc (M : List (Fml FF)) F :
   ⊢ sinv_auth_tok M ==∗ sinv_auth_tok (F :: M) ∗ sinv_tok (Pos.ofNat (List.length M)) F
 
-axiom sinv_tok_acc {i : Pos} {sm : cif FF -> Iris.IProp FF} {F : cif FF} :
+axiom sinv_tok_acc {i : Pos} {sm : Fml FF -> Iris.IProp FF} {F : Fml FF} :
   ⊢ sinv_tok i F -∗
     sinv_wsat sm -∗
     sm F ∗ (sm F -∗ sinv_wsat sm)
@@ -37,13 +37,13 @@ end sinv
 
 section inv
 
-def inv_tok (N : Namespace) (F : cif FF) : Iris.IProp FF :=
+def inv_tok (N : Namespace) (F : Fml FF) : Iris.IProp FF :=
   iprop(∃ i, ⌜i ∈ N⌝ ∗ sinv_tok i F)
 
-def magic_inv {sm : cif FF -> Iris.IProp FF} N F :=
+def magic_inv {sm : Fml FF -> Iris.IProp FF} N F :=
   iprop(∃ Q, (sm Q ∗-∗ sm F) ∗ inv_tok N F)
 
-theorem inv_tok_subset {N N'} {F : cif FF} :
+theorem inv_tok_subset {N N'} {F : Fml FF} :
   N ⊆ N' ->
   inv_tok N F ⊢ inv_tok N' F := by
   intros Hsubseteq
@@ -52,7 +52,7 @@ theorem inv_tok_subset {N N'} {F : cif FF} :
   iexists i; isplit; ipure_intro; apply (Hsubseteq Hin)
   iexact Hi
 
-axiom inv_tok_alloc {sm : cif FF -> Iris.IProp FF} (F : cif FF) N :
+axiom inv_tok_alloc {sm : Fml FF -> Iris.IProp FF} (F : Fml FF) N :
   ⊢ sm F ==∗ inv_tok N F
 
 end inv
