src/Iris/Nola/Notations.lean
@@ -2,26 +2,26 @@ import Iris.Nola.Syntax
 
 open Lean
 
--- define `cif` embedding in `term`
-syntax:max "cif(" term ")" : term
+-- define `fml` embedding in `term`
+syntax:max "fml(" term ")" : term
 syntax:max "term(" term ")" : term
 
 -- allow fallback to `term`
 macro_rules
-  | `(cif(term($t))) => pure t
-  | `(cif($t))       => pure t
+  | `(fml(term($t))) => pure t
+  | `(fml($t))       => pure t
 
--- carry `cif` over some `term` constructs
+-- carry `fml` over some `term` constructs
 macro_rules
-  | `(cif(($P)))                  => ``((cif($P)))
-  | `(cif(if $c then $t else $e)) => ``(if $c then cif($t) else cif($e))
-  | `(cif(($P : $t)))             => ``((cif($P) : $t))
+  | `(fml(($P)))                  => ``((fml($P)))
+  | `(fml(if $c then $t else $e)) => ``(if $c then fml($t) else fml($e))
+  | `(fml(($P : $t)))             => ``((fml($P) : $t))
 
-macro:max "cif(" P:term " : " t:term ")" : term => `((cif($P) : $t))
+macro:max "fml(" P:term " : " t:term ")" : term => `((fml($P) : $t))
 
-/-- Remove an `cif` quotation from a `term` syntax object. -/
+/-- Remove an `fml` quotation from a `term` syntax object. -/
 partial def unpackCif [Monad m] [MonadRef m] [MonadQuotation m] : Term → m Term
-  | `(cif($P))             => do `($P)
+  | `(fml($P))             => do `($P)
   | `($P:ident)              => do `($P)
   | `(?$P:ident)             => do `(?$P)
   | `(($P))                  => do `(($(← unpackCif P)))
@@ -33,90 +33,90 @@ partial def unpackCif [Monad m] [MonadRef m] [MonadQuotation m] : Term → m Ter
   | `(($P : $t))             => do ``(($(← unpackCif P) : $t))
   | `($t)                    => `($t:term)
 
--- `cif` syntax interpretation
+-- `fml` syntax interpretation
 macro_rules
-  | `(cif(⌜$φ⌝))      => ``(cif.pure $φ)
-  | `(cif($P ∧ $Q))   => ``(cif.and cif($P) cif($Q))
-  | `(cif($P ∨ $Q))   => ``(cif.or cif($P) cif($Q))
-  | `(cif($P → $Q))   => ``(cif.imp cif($P) cif($Q))
-  | `(cif(∃ $xs, $Ψ)) => do expandExplicitBinders ``cif.ex xs (← ``(cif($Ψ)))
-  | `(cif($P ∗ $Q))   => ``(cif.sep cif($P) cif($Q))
-  | `(cif($P -∗ $Q))  => ``(cif.wand cif($P) cif($Q))
-  | `(cif($P ∗-∗ $Q)) => ``(cif.wandIff cif($P) cif($Q))
-  | `(cif(<pers> $P)) => ``(cif.pers cif($P))
-  | `(cif(▷ $P))      => ``(cif.later cif($P))
-  | `(cif(|==> $P))  => ``(cif.bupd iprop($P))
-  | `(cif($P ==∗ $Q))  => ``(cif.wand iprop($P) (cif.bupd iprop($Q)))
-  | `(cif(■ $P))  => ``(cif.plain iprop($P))
+  | `(fml(⌜$φ⌝))      => ``(Fml.pure $φ)
+  | `(fml($P ∧ $Q))   => ``(Fml.and fml($P) fml($Q))
+  | `(fml($P ∨ $Q))   => ``(Fml.or fml($P) fml($Q))
+  | `(fml($P → $Q))   => ``(Fml.imp fml($P) fml($Q))
+  | `(fml(∃ $xs, $Ψ)) => do expandExplicitBinders ``Fml.ex xs (← ``(fml($Ψ)))
+  | `(fml($P ∗ $Q))   => ``(Fml.sep fml($P) fml($Q))
+  | `(fml($P -∗ $Q))  => ``(Fml.wand fml($P) fml($Q))
+  | `(fml($P ∗-∗ $Q)) => ``(Fml.wandIff fml($P) fml($Q))
+  | `(fml(<pers> $P)) => ``(Fml.pers fml($P))
+  | `(fml(▷ $P))      => ``(Fml.later fml($P))
+  | `(fml(|==> $P))  => ``(Fml.bupd iprop($P))
+  | `(fml($P ==∗ $Q))  => ``(Fml.wand iprop($P) (Fml.bupd iprop($Q)))
+  | `(fml(■ $P))  => ``(Fml.plain iprop($P))
 
-delab_rule cif.pure
-  | `($_ $φ) => ``(cif(⌜$φ⌝))
-delab_rule cif.and
-  | `($_ $P $Q) => do ``(cif($(← unpackCif P) ∧ $(← unpackCif Q)))
-delab_rule cif.or
-  | `($_ $P $Q) => do ``(cif($(← unpackCif P) ∨ $(← unpackCif Q)))
-delab_rule cif.imp
-  | `($_ $P $Q) => do ``(cif($(← unpackCif P) → $(← unpackCif Q)))
-delab_rule cif.all
-  | `($_ $_:term fun $x:ident => cif(∀ $y:ident $[$z:ident]*, $Ψ)) => do
-    ``(cif(∀ $x:ident $y:ident $[$z:ident]*, $Ψ))
-  | `($_ $_:term fun $x:ident => $Ψ) => do ``(cif(∀ $x:ident, $(← unpackCif Ψ)))
-delab_rule cif.ex
-  | `($_ $_:term fun $x:ident => cif(∃ $y:ident $[$z:ident]*, $Ψ)) => do
-    ``(cif(∃ $x:ident $y:ident $[$z:ident]*, $Ψ))
-  | `($_ $_:term fun $x:ident => $Ψ) => do ``(cif(∃ $x:ident, $(← unpackCif Ψ)))
-delab_rule cif.sep
-  | `($_ $P $Q) => do ``(cif($(← unpackCif P) ∗ $(← unpackCif Q)))
-delab_rule cif.wand
-  | `($_ $P $Q) => do ``(cif($(← unpackCif P) -∗ $(← unpackCif Q)))
-delab_rule cif.wandIff
-  | `($_ $P $Q) => do ``(cif($(← unpackCif P) ∗-∗ $(← unpackCif Q)))
-delab_rule cif.pers
-  | `($_ $P) => do ``(cif(<pers> $(← unpackCif P)))
-delab_rule cif.bupd
-  | `($_ $P) => do ``(cif(|==> $(← unpackCif P)))
-delab_rule cif.plain
-  | `($_ $P) => do ``(cif(■ $(← unpackCif P)))
+delab_rule Fml.pure
+  | `($_ $φ) => ``(fml(⌜$φ⌝))
+delab_rule Fml.and
+  | `($_ $P $Q) => do ``(fml($(← unpackCif P) ∧ $(← unpackCif Q)))
+delab_rule Fml.or
+  | `($_ $P $Q) => do ``(fml($(← unpackCif P) ∨ $(← unpackCif Q)))
+delab_rule Fml.imp
+  | `($_ $P $Q) => do ``(fml($(← unpackCif P) → $(← unpackCif Q)))
+delab_rule Fml.all
+  | `($_ $_:term fun $x:ident => fml(∀ $y:ident $[$z:ident]*, $Ψ)) => do
+    ``(fml(∀ $x:ident $y:ident $[$z:ident]*, $Ψ))
+  | `($_ $_:term fun $x:ident => $Ψ) => do ``(fml(∀ $x:ident, $(← unpackCif Ψ)))
+delab_rule Fml.ex
+  | `($_ $_:term fun $x:ident => fml(∃ $y:ident $[$z:ident]*, $Ψ)) => do
+    ``(fml(∃ $x:ident $y:ident $[$z:ident]*, $Ψ))
+  | `($_ $_:term fun $x:ident => $Ψ) => do ``(fml(∃ $x:ident, $(← unpackCif Ψ)))
+delab_rule Fml.sep
+  | `($_ $P $Q) => do ``(fml($(← unpackCif P) ∗ $(← unpackCif Q)))
+delab_rule Fml.wand
+  | `($_ $P $Q) => do ``(fml($(← unpackCif P) -∗ $(← unpackCif Q)))
+delab_rule Fml.wandIff
+  | `($_ $P $Q) => do ``(fml($(← unpackCif P) ∗-∗ $(← unpackCif Q)))
+delab_rule Fml.pers
+  | `($_ $P) => do ``(fml(<pers> $(← unpackCif P)))
+delab_rule Fml.bupd
+  | `($_ $P) => do ``(fml(|==> $(← unpackCif P)))
+delab_rule Fml.plain
+  | `($_ $P) => do ``(fml(■ $(← unpackCif P)))
 
-delab_rule cif.pure
-  | `($_ True) => ``(cif($(mkIdent `True)))
-  | `($_ False) => ``(cif($(mkIdent `False)))
-delab_rule cif.imp
-  | `($_ $P cif(False)) => do ``(cif(¬$(← unpackCif P)))
-  | `($_ $P $Q) => do ``(cif($(← unpackCif P) -> $(← unpackCif Q)))
+delab_rule Fml.pure
+  | `($_ True) => ``(fml($(mkIdent `True)))
+  | `($_ False) => ``(fml($(mkIdent `False)))
+delab_rule Fml.imp
+  | `($_ $P fml(False)) => do ``(fml(¬$(← unpackCif P)))
+  | `($_ $P $Q) => do ``(fml($(← unpackCif P) -> $(← unpackCif Q)))
 
 /- This is necessary since the `∀` syntax is not defined using `explicitBinders` and we can
 therefore not use `expandExplicitBinders` as for `∃`. -/
 macro_rules
-  | `(cif(∀ _%$tk, $Ψ)) => ``(cif.all (fun _%$tk => cif($Ψ)))
+  | `(fml(∀ _%$tk, $Ψ)) => ``(Fml.all (fun _%$tk => fml($Ψ)))
 macro_rules
-  | `(cif(∀ $x:ident, $Ψ)) => ``(cif.all (fun $x => cif($Ψ)))
+  | `(fml(∀ $x:ident, $Ψ)) => ``(Fml.all (fun $x => fml($Ψ)))
 macro_rules
-  | `(cif(∀ (_%$tk : $t), $Ψ)) => ``(cif.all (fun (_%$tk : $t) => cif($Ψ)))
-  | `(cif(∀ (_%$tk $xs* : $t), $Ψ)) =>
-    ``(cif.all (fun (_%$tk : $t) => cif(∀ ($xs* : $t), $Ψ)))
+  | `(fml(∀ (_%$tk : $t), $Ψ)) => ``(Fml.all (fun (_%$tk : $t) => fml($Ψ)))
+  | `(fml(∀ (_%$tk $xs* : $t), $Ψ)) =>
+    ``(Fml.all (fun (_%$tk : $t) => fml(∀ ($xs* : $t), $Ψ)))
 macro_rules
-  | `(cif(∀ ($x:ident : $t), $Ψ)) => ``(cif.all (fun ($x : $t) => cif($Ψ)))
-  | `(cif(∀ ($x:ident $xs* : $t), $Ψ)) =>
-    ``(cif.all (fun ($x : $t) => cif(∀ ($xs* : $t), $Ψ)))
+  | `(fml(∀ ($x:ident : $t), $Ψ)) => ``(Fml.all (fun ($x : $t) => fml($Ψ)))
+  | `(fml(∀ ($x:ident $xs* : $t), $Ψ)) =>
+    ``(Fml.all (fun ($x : $t) => fml(∀ ($xs* : $t), $Ψ)))
 macro_rules
-  | `(cif(∀ {_%$tk : $t}, $Ψ)) =>
-    ``(cif.all (fun {_%$tk : $t}  => cif($Ψ)))
-  | `(cif(∀ {_%$tk $xs* : $t}, $Ψ)) =>
-    ``(cif.all (fun {_%$tk : $t}  => cif(∀ {$xs* : $t}, $Ψ)))
+  | `(fml(∀ {_%$tk : $t}, $Ψ)) =>
+    ``(Fml.all (fun {_%$tk : $t}  => fml($Ψ)))
+  | `(fml(∀ {_%$tk $xs* : $t}, $Ψ)) =>
+    ``(Fml.all (fun {_%$tk : $t}  => fml(∀ {$xs* : $t}, $Ψ)))
 macro_rules
-  | `(cif(∀ {$x:ident : $t}, $Ψ)) =>
-    ``(cif.all (fun ($x : $t) => cif($Ψ)))
-  | `(cif(∀ {$x:ident $xs* : $t}, $Ψ)) =>
-    ``(cif.all (fun ($x : $t) => cif(∀ {$xs* : $t}, $Ψ)))
+  | `(fml(∀ {$x:ident : $t}, $Ψ)) =>
+    ``(Fml.all (fun ($x : $t) => fml($Ψ)))
+  | `(fml(∀ {$x:ident $xs* : $t}, $Ψ)) =>
+    ``(Fml.all (fun ($x : $t) => fml(∀ {$xs* : $t}, $Ψ)))
 macro_rules
-  | `(cif(∀ $x $y $xs*, $Ψ)) => ``(cif(∀ $x, ∀ $y $xs*, $Ψ))
+  | `(fml(∀ $x $y $xs*, $Ψ)) => ``(fml(∀ $x, ∀ $y $xs*, $Ψ))
 
--- `cif` macros
+-- `fml` macros
 macro_rules
-  | `(cif(True))  => ``(cif.pure True)
-  | `(cif(False)) => ``(cif.pure False)
-  | `(cif(¬$P))   => ``(cif($P → False))
+  | `(fml(True))  => ``(Fml.pure True)
+  | `(fml(False)) => ``(Fml.pure False)
+  | `(fml(¬$P))   => ``(fml($P → False))
 
 /-- Intuitionistic modality.
 ```
@@ -125,22 +125,22 @@ def intuitionistically (P) := <affine> <pers> P
 -/
 
 macro_rules
-  | `(cif(◇ $P)) => ``(cif.except0 cif($P))
+  | `(fml(◇ $P)) => ``(Fml.except0 fml($P))
 
-delab_rule cif.except0
-  | `($_ $P) => do ``(cif(◇ $(← unpackCif P)))
+delab_rule Fml.except0
+  | `($_ $P) => do ``(fml(◇ $(← unpackCif P)))
 
-def testCif1 : cif FF :=
-  cif.all (fun (x : Nat) => cif.all (fun (y : Nat) => cif.pure (x < y)))
+def testCif1 : Fml FF :=
+  Fml.all (fun (x : Nat) => Fml.all (fun (y : Nat) => Fml.pure (x < y)))
 
 #print testCif1
 
-def testCif2 : cif FF :=
-  cif(∀ (x : Nat), ⌜x = 1⌝)
+def testCif2 : Fml FF :=
+  fml(∀ (x : Nat), ⌜x = 1⌝)
 
 #print testCif2
 
-def testCif3 : cif FF :=
-  cif(∀ x (y : Nat), ⌜x < y⌝ -> ⌜¬ x ≥ y⌝)
+def testCif3 : Fml FF :=
+  fml(∀ x (y : Nat), ⌜x < y⌝ -> ⌜¬ x ≥ y⌝)
 
 #print testCif3
